@@ -378,24 +378,23 @@ theorem wp_m_jal (cpu : CPU) (dq : DFrac) (c : MConf) (hok : MConf.ok (GF := GF)
 
 /-- `ld rd, imm(rd)` from an 8-aligned RAM address. -/
 theorem wp_m_ld_same [CurCtx] (cpu : CPU) (dq dq' : DFrac) (c : MConf) (hok : MConf.ok (GF := GF) c)
-    (hct : curTier = KTier.bare)
     (pc : BitVec 64) (is_rvc : Bool)
     (imm : BitVec 12) (rd : BitVec 5) (hrd : rd ≠ 0#5) (a data : BitVec 64) :
     instr (GF := GF) pc is_rvc (instruction.LOAD (imm, regidx.Regidx rd, regidx.Regidx rd, false, 8)) ∗
     mConf cpu dq c ∗ clockCells cpu ∗ pcIs cpu pc ∗ gpr cpu rd (DFrac.own 1) a ∗ ctxTok cpu curCtx ∗
-    wordPointsTo (a + BitVec.signExtend 64 imm) 8 dq' data ∗
+    pwordPointsTo (a + BitVec.signExtend 64 imm) 8 dq' data ∗
     ▷ (mConf cpu dq c -∗ clockCells cpu -∗ pcIs cpu (pc + instrLen is_rvc) -∗
         gpr cpu rd (DFrac.own 1) data -∗ ctxTok cpu curCtx -∗
-        wordPointsTo (a + BitVec.signExtend 64 imm) 8 dq' data -∗ wpLoop cpu)
+        pwordPointsTo (a + BitVec.signExtend 64 imm) 8 dq' data -∗ wpLoop cpu)
     ⊢ wpLoop cpu := by
   iintro ⟨HI, HmConf, Hclock, Hpc, Hrd, Htok, Hw, HΦ⟩
-  icases wordPointsTo_bare_acc _ _ _ _ hct $$ Hw with ⟨%⟨hram, hal⟩, #Hcl, Hbytes⟩
+  icases pwordPointsTo_cases _ _ _ _ $$ Hw with ⟨%⟨hram, hal⟩, Hbytes⟩
   iapply wpLoop_m_instr cpu dq c c hok pc _ is_rvc _ _ _
     (execSpec_ld_same cpu dq dq' c hok pc _ imm rd hrd a data hram hal)
   iframe
   inext
   iintro HmConf Hclock Hpc ⟨Hrd, Htok, Hbytes⟩
-  ihave Hw := wordPointsTo_intro_id _ _ _ _ hram hal $$ Hcl Hbytes
+  ihave Hw := pwordPointsTo_intro _ _ _ _ hram hal $$ Hbytes
   iapply HΦ $$ HmConf Hclock Hpc Hrd Htok Hw
 
 end MachCSL
